

$$\begin{aligned} (4) \quad dy &= \frac{y}{x} dx \\ &= \left(\frac{1}{1 + \frac{1}{x^2}} \right) \cdot \left(\frac{y}{\frac{1}{x^2}} \right) \cdot (-x^2) dx \\ &= \left(\frac{x}{(1 + x^2)^2} \right) dx \\ (5) \quad \int \frac{1}{x^2} e^{\frac{1}{x}} dx &= \int \frac{1}{x^2} e^u \cdot (-\frac{1}{x^2}) dx \end{aligned}$$

(b) $x dy^2 + y^2 dx = x^2 dy + y dx^2 = 0$

4. (i) $e^{a+b} \approx 1 + a + \frac{a^2}{2} + \dots$

(ii) $\int_{-1}^1 \frac{1}{\sqrt{1-x^2}} = \frac{1}{\sqrt{1-1}} - \frac{1}{\sqrt{1-(-1)^2}} = \frac{1}{\sqrt{0}} - \frac{1}{\sqrt{0}} = \infty - \infty$

5. (i) $\frac{d^2 y}{dx^2} = 0$

(ii) $\frac{d}{dx} \left(\frac{1}{x^2} \right) = -\frac{2}{x^3}$

(iii) $\frac{d}{dx} \cos x = -\sin x$

(iv) $\frac{d}{dx} (x^2) = 2x$

(1b) $\lim_{x \rightarrow 10} \frac{1}{x} \ln(\ln(x))$ $\lim_{x \rightarrow 10} \frac{\frac{1}{x} \cdot \frac{1}{x}}{\frac{1}{x}}$ $\lim_{x \rightarrow 10} \frac{\frac{1}{x^2}}{\frac{1}{x}}$

$\lim_{x \rightarrow 10} \frac{\ln(\ln(x))}{x-10}$ $\lim_{x \rightarrow 10} \frac{\frac{1}{x} \cdot \frac{1}{x}}{1}$ $\lim_{x \rightarrow 10} \frac{1}{x^2} = \frac{1}{100}$ ✓

(1c) $\lim_{x \rightarrow 1} \frac{e^{3x}-1}{e^{3x+1}} = \lim_{x \rightarrow 1} \frac{3e^{3x}}{e^{3x+1}} = 3$ ✓

(1d) $\lim_{x \rightarrow 0} \frac{1 - \frac{\cos x}{1 + \frac{\cos x}{x}}}{1 + \frac{\cos x}{x}} = 1$ ✓

2. $\lim_{x \rightarrow 0} \frac{f(x)-2}{x} = \lim_{x \rightarrow 0} \frac{f(x)}{x} = \frac{2}{1} = 2$ ✓

(b) $y' = \frac{1}{2}x^{-\frac{1}{2}} + \frac{1}{2}(x-1)x^{-\frac{1}{2}}$
 $y'' = -\frac{1}{4}x^{-\frac{3}{2}} + \frac{1}{4}(x-1)^{-\frac{1}{2}} - \frac{1}{4}x^{-\frac{1}{2}}$
 $= -\frac{1}{4}x^{-\frac{3}{2}} + \frac{1}{4\sqrt{x-1}} - \frac{1}{4}x^{-\frac{1}{2}}$
 $y''(0.01) = \frac{1}{4\sqrt{0.01}}(0.01 - \frac{1}{4}) - \frac{1}{4}(0.01)^{-\frac{1}{2}}$
 $= \frac{1}{4\sqrt{0.01}}(-0.25) - \frac{1}{4\sqrt{0.01}}$
 $= \frac{1}{4\sqrt{0.01}}(-0.5) = -\frac{1}{8\sqrt{0.01}} = -\frac{1}{8 \cdot 0.1} = -\frac{1}{0.8} = -1.25$

[illegible]



$$(1) \int_0^1 \ln(x+1) dx = \frac{1}{2} x^2 \ln(x+1) - \int_0^1 \frac{1}{2} x^2 \cdot \frac{1}{x+1} dx$$

$$= \frac{1}{2} x^2 \ln(x+1) - \frac{1}{2} \int_0^1 x^2 \ln(x+1) dx + \frac{1}{2} \int_0^1 \frac{x^2}{x+1} dx$$

$$= \frac{1}{2} x^2 \ln(x+1) - \frac{1}{2} (x^2)^2 - \frac{1}{2} \ln|x+1| + C$$

$$(2) \int_0^1 x^2 \ln(x+1) dx = \int_0^1 x^2 (1 + \cos x) dx = \int_0^1 x^2 dx + \int_0^1 x^2 \cos x dx$$

$$= \frac{1}{3} x^3 + \frac{1}{3} x^2 \sin x - \frac{1}{3} \int_0^1 x \sin x dx$$

$$= \frac{1}{3} x^3 + \frac{1}{3} x^2 \sin x - \frac{1}{3} \int_0^1 x \sin x dx$$

$$= \frac{1}{3} x^3 + \frac{1}{3} x^2 \sin x - \frac{1}{3} \int_0^1 x \sin x dx$$

$$(3) \int_0^1 \ln(x+1) dx = -\frac{1}{2} \ln 2 + \int_0^1 \ln(x+1) dx$$

$$= -\frac{1}{2} \ln 2 + \int_0^1 \ln(x+1) dx$$

$$= -\frac{1}{2} \ln 2 + \int_0^1 \ln(x+1) dx$$

$$= -\frac{1}{2} \ln 2 + \int_0^1 \ln(x+1) dx$$

$$(4) -\frac{1}{2} \ln 2 - \frac{1}{2} \ln 2 - \frac{1}{2} \ln 2 + \frac{1}{2} \ln 2 + C$$

$$(4) \int_0^1 x \ln(x+1) dx = \frac{1}{2} x^2 \ln(x+1) - \frac{1}{2} \int_0^1 x^2 \ln(x+1) dx$$

$$= \frac{1}{2} x^2 \ln(x+1) - \frac{1}{2} \int_0^1 x^2 \ln(x+1) dx$$

$$(5) \int_0^1 \ln(x+1) dx = \int_0^1 \ln(x+1) dx = \ln(x+1) - \int_0^1 \frac{1}{x+1} dx$$

$$= \ln(x+1) - \ln|x+1| + C$$

$$= \ln(x+1) - \ln|x+1| + C$$

$$(6) \int_0^1 \frac{x e^x}{x+1} dx = \int_0^1 x e^x dx - \int_0^1 \frac{x e^x}{x+1} dx$$

$$= \frac{x e^x}{x+1} + \int_0^1 \frac{1}{x+1} dx$$

$$= \frac{x e^x}{x+1} + \int_0^1 \frac{1}{x+1} dx$$

$$= \frac{x e^x}{x+1} + \int_0^1 \frac{1}{x+1} dx$$

$$= \frac{x e^x}{x+1} + \int_0^1 \frac{1}{x+1} dx$$

$$= \frac{x e^x}{x+1} + \int_0^1 \frac{1}{x+1} dx$$

$$= \frac{x e^x}{x+1} + \int_0^1 \frac{1}{x+1} dx$$

$$= \frac{x e^x}{x+1} + \int_0^1 \frac{1}{x+1} dx$$

$$= \frac{x e^x}{x+1} + \int_0^1 \frac{1}{x+1} dx$$